LeanMachines/Refinement/Bidirectional/Basic.lean
@@ -4,7 +4,7 @@ import LeanMachines.Refinement.Strong.Basic
 
 class BiRefinement {ACTX : outParam (Type u₁)} (AM)
                  {CTX : outParam (Type u₂)} (M)
-                 [Machine ACTX AM] [Machine CTX M] extends SRefinement AM M where
+                 [@Machine ACTX AM] [@Machine CTX M] extends SRefinement AM M where
 
   unlift_lift  (m m' : M):
     Machine.invariant m
