LeanMachines/Refinement/Functional/NonDet/Convergent.lean
@@ -6,49 +6,49 @@ open Refinement
 open FRefinement
 
 @[simp]
-def newAnticipatedFRNDEventfromOrdinary [Preorder v] [Machine ACTX AM] [Machine CTX M] [FRefinement AM M]
+def newAnticipatedFRNDEventfromOrdinary [Preorder v] [@Machine ACTX AM] [@Machine CTX M] [FRefinement AM M]
   (abs : OrdinaryNDEvent AM α' β')
   (ev : AnticipatedRNDEventSpec v AM M (α:=α) (β:=β) (α':=α') (β':=β') abs) : AnticipatedRNDEvent v AM M α β α' β' :=
   newAnticipatedRNDEventfromOrdinary abs ev
 
 @[simp]
-def newAnticipatedFRNDEventfromOrdinary' [Preorder v] [Machine ACTX AM] [Machine CTX M] [FRefinement AM M]
+def newAnticipatedFRNDEventfromOrdinary' [Preorder v] [@Machine ACTX AM] [@Machine CTX M] [FRefinement AM M]
   (abs : OrdinaryNDEvent AM α' Unit)
   (ev : AnticipatedRNDEventSpec' v AM M (α:=α) (α':=α') abs) : AnticipatedRNDEvent v AM M α Unit α' Unit :=
   newAnticipatedRNDEventfromOrdinary abs ev.toAnticipatedRNDEventSpec
 
 @[simp]
-def newAnticipatedFRNDEventfromOrdinary'' [Preorder v] [Machine ACTX AM] [Machine CTX M] [FRefinement AM M]
+def newAnticipatedFRNDEventfromOrdinary'' [Preorder v] [@Machine ACTX AM] [@Machine CTX M] [FRefinement AM M]
   (abs : OrdinaryNDEvent AM Unit Unit)
   (ev : AnticipatedRNDEventSpec'' v AM M abs) : AnticipatedRNDEvent v AM M Unit Unit :=
   newAnticipatedRNDEventfromOrdinary abs ev.toAnticipatedRNDEventSpec
 
 @[simp]
-def newAnticipatedFRNDEventfromAnticipated [Preorder v] [Machine ACTX AM] [Machine CTX M] [FRefinement AM M]
+def newAnticipatedFRNDEventfromAnticipated [Preorder v] [@Machine ACTX AM] [@Machine CTX M] [FRefinement AM M]
   (abs : AnticipatedNDEvent v AM α' β') (ev : AnticipatedRNDEventSpec v AM M (α:=α) (β:=β) (α':=α') (β':=β') abs.toOrdinaryNDEvent) : AnticipatedRNDEvent v AM M α β α' β' :=
   newAnticipatedRNDEventfromAnticipated abs ev
 
 @[simp]
-def newAnticipatedFRNDEventfromAnticipated' [Preorder v] [Machine ACTX AM] [Machine CTX M] [FRefinement AM M]
+def newAnticipatedFRNDEventfromAnticipated' [Preorder v] [@Machine ACTX AM] [@Machine CTX M] [FRefinement AM M]
   (abs : AnticipatedNDEvent v AM α' Unit) (ev : AnticipatedRNDEventSpec' v AM M (α:=α) (α':=α') abs.toOrdinaryNDEvent) : AnticipatedRNDEvent v AM M α Unit α' Unit :=
   newAnticipatedRNDEventfromAnticipated abs ev.toAnticipatedRNDEventSpec
 
 @[simp]
-def newAnticipatedFRNDEventfromAnticipated'' [Preorder v] [Machine ACTX AM] [Machine CTX M] [FRefinement AM M]
+def newAnticipatedFRNDEventfromAnticipated'' [Preorder v] [@Machine ACTX AM] [@Machine CTX M] [FRefinement AM M]
   (abs : AnticipatedNDEvent v AM Unit Unit) (ev : AnticipatedRNDEventSpec'' v AM M abs.toOrdinaryNDEvent) : AnticipatedRNDEvent v AM M Unit Unit :=
   newAnticipatedRNDEventfromAnticipated abs ev.toAnticipatedRNDEventSpec
 
 @[simp]
-def newConvergentFRNDEvent [Preorder v] [WellFoundedLT v] [Machine ACTX AM] [Machine CTX M] [FRefinement AM M]
+def newConvergentFRNDEvent [Preorder v] [WellFoundedLT v] [@Machine ACTX AM] [@Machine CTX M] [FRefinement AM M]
   (abs : OrdinaryNDEvent AM α' β') (ev : ConvergentRNDEventSpec v AM M (α:=α) (β:=β) (α':=α') (β':=β') abs) : ConvergentRNDEvent v AM M α β α' β' :=
   newConvergentRNDEvent abs ev
 
 @[simp]
-def newConvergentFRNDEvent' [Preorder v] [WellFoundedLT v] [Machine ACTX AM] [Machine CTX M] [FRefinement AM M]
+def newConvergentFRNDEvent' [Preorder v] [WellFoundedLT v] [@Machine ACTX AM] [@Machine CTX M] [FRefinement AM M]
   (abs : OrdinaryNDEvent AM α' Unit) (ev : ConvergentRNDEventSpec' v AM M (α:=α) (α':=α') abs) : ConvergentRNDEvent v AM M α Unit α' Unit :=
   newConvergentRNDEvent abs ev.toConvergentRNDEventSpec
 
 @[simp]
-def newConvergentFRNDEvent'' [Preorder v] [WellFoundedLT v] [Machine ACTX AM] [Machine CTX M] [FRefinement AM M]
+def newConvergentFRNDEvent'' [Preorder v] [WellFoundedLT v] [@Machine ACTX AM] [@Machine CTX M] [FRefinement AM M]
   (abs : OrdinaryNDEvent AM Unit Unit) (ev : ConvergentRNDEventSpec'' v AM M abs) : ConvergentRNDEvent v AM M Unit Unit :=
   newConvergentRNDEvent abs ev.toConvergentRNDEventSpec
