LeanMachines/Refinement/Strong/Concrete.lean
@@ -7,17 +7,17 @@ open FRefinement
 open SRefinement
 
 @[simp]
-def newConcreteSREvent [Machine ACTX AM] [Machine CTX M] [SRefinement AM M]
+def newConcreteSREvent [@Machine ACTX AM] [@Machine CTX M] [SRefinement AM M]
    (ev : ConcreteFREventSpec AM M α β) : OrdinaryRDetEvent AM M α β :=
   newConcreteFREvent ev
 
 @[simp]
-def newConcreteSREvent' [Machine ACTX AM] [Machine CTX M] [SRefinement AM M]
+def newConcreteSREvent' [@Machine ACTX AM] [@Machine CTX M] [SRefinement AM M]
    (ev : ConcreteFREventSpec' AM M α) : OrdinaryRDetEvent AM M α Unit :=
   newConcreteFREvent ev.toConcreteFREventSpec
 
 @[simp]
-def newConcreteSREvent'' [Machine ACTX AM] [Machine CTX M] [SRefinement AM M]
+def newConcreteSREvent'' [@Machine ACTX AM] [@Machine CTX M] [SRefinement AM M]
    (ev : ConcreteFREventSpec'' AM M) : OrdinaryRDetEvent AM M Unit Unit :=
   newConcreteFREvent ev.toConcreteFREventSpec
 
@@ -25,19 +25,19 @@ def newConcreteSREvent'' [Machine ACTX AM] [Machine CTX M] [SRefinement AM M]
 
 @[simp]
 def newConcreteAnticipatedSREvent [Preorder v] [WellFoundedLT v]
-                       [Machine ACTX AM] [Machine CTX M] [SRefinement AM M]
+                       [@Machine ACTX AM] [@Machine CTX M] [SRefinement AM M]
    (ev : ConcreteAnticipatedFREventSpec v AM M α β) : AnticipatedRDetEvent v AM M α β :=
   newConcreteAnticipatedFREvent ev
 
 @[simp]
 def newConcreteAnticipatedSREvent' [Preorder v] [WellFoundedLT v]
-                       [Machine ACTX AM] [Machine CTX M] [SRefinement AM M]
+                       [@Machine ACTX AM] [@Machine CTX M] [SRefinement AM M]
    (ev : ConcreteAnticipatedFREventSpec' v AM M α) : AnticipatedRDetEvent v AM M α Unit :=
   newConcreteAnticipatedREvent ev.toConcreteAnticipatedREventSpec
 
 @[simp]
 def newConcreteAnticipatedSREvent'' [Preorder v] [WellFoundedLT v]
-                       [Machine ACTX AM] [Machine CTX M] [SRefinement AM M]
+                       [@Machine ACTX AM] [@Machine CTX M] [SRefinement AM M]
    (ev : ConcreteAnticipatedFREventSpec'' v AM M) : AnticipatedRDetEvent v AM M Unit Unit :=
   newConcreteAnticipatedFREvent ev.toConcreteAnticipatedFREventSpec
 
@@ -46,18 +46,18 @@ def newConcreteAnticipatedSREvent'' [Preorder v] [WellFoundedLT v]
 
 @[simp]
 def newConcreteConvergentSREvent [Preorder v] [WellFoundedLT v]
-                       [Machine ACTX AM] [Machine CTX M] [SRefinement AM M]
+                       [@Machine ACTX AM] [@Machine CTX M] [SRefinement AM M]
    (ev : ConcreteConvergentFREventSpec v AM M α β) : ConvergentRDetEvent v AM M α β :=
   newConcreteConvergentFREvent ev
 
 @[simp]
 def newConcreteConvergentSREvent' [Preorder v] [WellFoundedLT v]
-                       [Machine ACTX AM] [Machine CTX M] [SRefinement AM M]
+                       [@Machine ACTX AM] [@Machine CTX M] [SRefinement AM M]
    (ev : ConcreteConvergentFREventSpec' v AM M α) : ConvergentRDetEvent v AM M α Unit :=
   newConcreteConvergentREvent ev.toConcreteConvergentREventSpec
 
 @[simp]
 def newConcreteConvergentSREvent'' [Preorder v] [WellFoundedLT v]
-                       [Machine ACTX AM] [Machine CTX M] [SRefinement AM M]
+                       [@Machine ACTX AM] [@Machine CTX M] [SRefinement AM M]
    (ev : ConcreteConvergentFREventSpec'' v AM M) : ConvergentRDetEvent v AM M Unit Unit :=
   newConcreteConvergentFREvent ev.toConcreteConvergentFREventSpec
